K

example/Bellman_Ford.thy
@@ -19,7 +19,7 @@ fun bf :: "nat\<times>nat \<Rightarrow> int" where
     fold
       min
       (map
-        (\<lambda>i. plus (id (\<lambda>i'. bf (k, i')) i) (W i j))
+        (\<lambda>i. plus (W i j) (bf (k, i)))
         (upt 0 n))
       (bf (k, j))"
 thm bf.simps
@@ -31,69 +31,92 @@ fun bf\<^sub>T :: "nat\<times>nat \<Rightarrow>\<^sub>T int" where
     \<langle>fold\<^sub>T\<rangle>
     . \<langle>min\<^sub>T\<rangle>
     . (\<langle>map\<^sub>T\<rangle>
-      . \<langle>\<lambda>i. \<langle>plus\<^sub>T\<rangle> . (id (\<lambda>i'. bf\<^sub>T (k, i')) i) . \<langle>W i j\<rangle>\<rangle>
+      . \<langle>\<lambda>i. \<langle>plus\<^sub>T\<rangle> . \<langle>W i j\<rangle> . (bf\<^sub>T (k, i))\<rangle>
       . (\<langle>upt\<^sub>T\<rangle> . \<langle>0\<rangle> . \<langle>n\<rangle>))
     . (bf\<^sub>T (k, j))"
-
 term 0 (**)
-thm bf\<^sub>T.induct
   
 interpretation bf: dp_consistency bf .
-
 context
   includes lifting_syntax
 begin
 
+definition K :: "'a \<Rightarrow> 'a \<Rightarrow> 'a \<Rightarrow> bool" where
+  "K x \<equiv> \<lambda> a b. a=x \<and> b=x"
+term 0 (**)
+
 lemma bf_induct:
   "\<lbrakk>\<And>j. P (0, j);
-    \<And>k j. \<lbrakk>\<And>(x::nat) i. P (k, i);
-            P (k, j)
+    \<And>k j. \<lbrakk>\<And>x. P (k, x);
+           P (k, j)
            \<rbrakk> \<Longrightarrow> P (Suc k, j)
-    \<rbrakk> \<Longrightarrow> P (x::nat\<times>nat)"
+   \<rbrakk> \<Longrightarrow> P (x::nat\<times>nat)"
   by (fact bf\<^sub>T.induct)
 
 lemma bf_inductS:
   "\<lbrakk>\<And>j. bf.consistentS op = (bf (0, j)) (bf\<^sub>T (0, j));
-    \<And>k j. \<lbrakk>(op = ===> bf.consistentS op =) (\<lambda>i. bf (k, i)) (\<lambda>i. bf\<^sub>T (k, i));
-            bf.consistentS op = (bf (k, j)) (bf\<^sub>T (k, j))
+    \<And>k j. \<lbrakk>\<And>x. bf.consistentS op = (bf (k, x)) (bf\<^sub>T (k, x));
+           bf.consistentS op = (bf (k, j)) (bf\<^sub>T (k, j))
            \<rbrakk> \<Longrightarrow> bf.consistentS op = (bf (Suc k, j)) (bf\<^sub>T (Suc k, j))
-    \<rbrakk> \<Longrightarrow> bf.consistentS op = (bf (x::nat\<times>nat)) (bf\<^sub>T x)"
-  unfolding rel_fun_def by (metis bf_induct[of "\<lambda>x. bf.consistentS op = (bf x) (bf\<^sub>T x)"])
-  
-term 0 (**)
+   \<rbrakk> \<Longrightarrow> bf.consistentS op = (bf (x::nat\<times>nat)) (bf\<^sub>T x)"
+  by (fact bf_induct)
+
+lemma bf_inductS':
+  "\<lbrakk>\<And>j. bf.consistentS op = (bf (0, j)) (bf\<^sub>T (0, j));
+    \<And>k j. \<lbrakk>K k k k;
+           K j j j;
+           (rel_prod (K k) op = ===> bf.consistentS op =) bf bf\<^sub>T;
+           (rel_prod (K k) (K j) ===> bf.consistentS op =) bf bf\<^sub>T
+           \<rbrakk> \<Longrightarrow> bf.consistentS op = (bf (Suc k, j)) (bf\<^sub>T (Suc k, j))
+   \<rbrakk> \<Longrightarrow> bf.consistentS op = (bf (x::nat\<times>nat)) (bf\<^sub>T x)"
+  unfolding rel_prod.simps rel_fun_def K_def by (simp add: bf_inductS)
+  term 0 (**)
+
+  term 0 (**)
 lemma "bf.consistentDP bf\<^sub>T"
-proof ((rule bf.consistentDP_intro, induct_tac rule: bf_inductS, unfold bf\<^sub>T.simps; rule bf.consistentS_checkmem, unfold bf.simps), goal_cases)
-  case [transfer_rule]: 1 show ?case by transfer_prover
-next
-  case prems[transfer_rule]: (2 _ k j)
-    show ?case
-      apply transfer_prover_start
-                          apply transfer_step
-      apply transfer_step
-                          apply transfer_step
-      apply transfer_step
-      apply transfer_step
-                          apply transfer_step
-      apply transfer_step
-                          apply transfer_step
-                          apply transfer_step
-      apply transfer_step
-                          apply transfer_step
-                          apply transfer_step
-                          apply transfer_step
-                         apply transfer_step
-                        apply transfer_step
-                       apply transfer_step
-                      apply transfer_step
-                     apply transfer_step
-        apply transfer_step
-    term 0 (**
-  subgoal premises [transfer_rule] by transfer_prover
-  subgoal premises prems[transfer_rule]
-    apply transfer
-      
+  apply (rule bf.consistentDP_intro, induct_tac rule: bf_inductS', unfold bf\<^sub>T.simps; rule bf.consistentS_checkmem, unfold bf.simps)
+  subgoal premises prems[transfer_rule] by transfer_prover
+  subgoal premises prems
     thm prems
+supply [transfer_rule] = prems(1)
     apply transfer_prover_start
+      (*
+                        defer
+                        defer
+                        defer
+                        defer
+                        defer
+                        defer
+                        defer
+                        defer
+                        defer
+                        defer
+                        defer
+                        defer
+                        defer
+                        defer
+                        defer
+                        defer
+                        defer
+                        defer
+                        defer
+                        defer
+                        defer
+                        defer
+                        defer
+                        defer
+                        defer
+                        defer
+                        defer
+                        defer
+                        defer
+                        defer
+                        defer
+*)
+    oops
+lemma 
+  assumes "R "
+      term 0 (**
                         apply transfer_step
                         apply transfer_step
                         apply transfer_step
@@ -102,13 +125,12 @@ next
                         apply transfer_step
                         apply transfer_step
                         apply transfer_step
-      
-                        
-      
+                        apply transfer_step
+                        apply transfer_step
+                        apply transfer_step
+                        apply transfer_step
+      thm prems
       (* going wrong here *)
       (* bf\<^sub>T (Pair k i) should be proved directly by prems(1) rather than be separated *)
-    thm prems
     oops
-    thm bf.induct bf\<^sub>T.induct
-      thm bf_induct[of "\<lambda>x. bf.consistentS op = (bf x) (bf\<^sub>T x)"]
 end
